Finished proof about length of proof_forest

Congruence_Closure_Explain/CC_Abstraction.thy
@@ -64,12 +64,25 @@ fun valid_vars :: "equation \<Rightarrow> nat \<Rightarrow> bool"
     "valid_vars (a \<approx> b) n = (a < n \<and> b < n)"
   | "valid_vars (F a b \<approx> c) n = (a < n \<and> b < n \<and> c < n)"
 
-fun valid_vars_pending :: "pending_equation \<Rightarrow> nat list \<Rightarrow> nat \<Rightarrow> bool"
+fun valid_vars_pending :: "pending_equation \<Rightarrow> nat \<Rightarrow> bool"
   where
-    "valid_vars_pending (One (a \<approx> b)) pf n = (valid_vars (a \<approx> b) n)"
-  | "valid_vars_pending (Two (F a\<^sub>1 a\<^sub>2 \<approx> a) (F b\<^sub>1 b\<^sub>2 \<approx> b)) pf n = 
+    "valid_vars_pending (One (a \<approx> b)) n = (valid_vars (a \<approx> b) n)"
+  | "valid_vars_pending (Two (F a\<^sub>1 a\<^sub>2 \<approx> a) (F b\<^sub>1 b\<^sub>2 \<approx> b)) n = 
         (valid_vars (F a\<^sub>1 a\<^sub>2 \<approx> a) n \<and> valid_vars (F b\<^sub>1 b\<^sub>2 \<approx> b) n)"
-  | "valid_vars_pending _ _ _ = False"
+  | "valid_vars_pending _ _ = False"
+
+lemma valid_vars_pendingI: 
+  "valid_vars_pending a n \<longleftrightarrow> (\<exists> b c . b < n \<and> c < n \<and> a = (One (b \<approx> c))) \<or>
+(\<exists> b c d e f g . b < n \<and> c < n \<and> d < n \<and> e < n \<and> f < n \<and> g < n \<and> a = (Two (F b c \<approx> d) (F e f \<approx> g)))"
+  (is "?P \<longleftrightarrow> ?Q")
+proof
+  show "?P \<Longrightarrow> ?Q" apply(cases a) 
+    using valid_vars_pending.elims(2) apply fastforce 
+    using valid_vars_pending.elims by (metis pending_equation.distinct(1) valid_vars.simps(2))
+  show "?Q \<Longrightarrow> ?P"
+    apply(cases a) 
+    by auto
+qed
 
 abbreviation nr_vars :: "congruence_closure \<Rightarrow> nat"
   where
@@ -89,20 +102,28 @@ text \<open>for each representative i, UseList (i) is a list of input equations 
 such that i is the representative of \<open>b\<^sub>1\<close> or of \<open>b\<^sub>2\<close> (or of both).\<close>
 abbreviation use_list_invar_correctness :: "congruence_closure \<Rightarrow> bool"
   where
-    "use_list_invar_correctness cc \<equiv> (\<forall> i < nr_vars cc . (\<forall> j < length ((use_list cc) ! i) . 
-(cc_list cc) ! i = i \<longrightarrow> (\<exists> b\<^sub>1 b\<^sub>2 b .
-use_list cc ! i ! j = (F b\<^sub>1 b\<^sub>2 \<approx> b) \<and> 
-(i = rep_of (cc_list cc) b\<^sub>1) \<or> i = rep_of (cc_list cc) b\<^sub>2)))"
+    "use_list_invar_correctness cc \<equiv> 
+(\<forall> i < nr_vars cc . 
+  (\<forall> j < length ((use_list cc) ! i) . (cc_list cc) ! i = i \<longrightarrow> 
+    (\<exists> b\<^sub>1 b\<^sub>2 b . use_list cc ! i ! j = (F b\<^sub>1 b\<^sub>2 \<approx> b) \<and> 
+      ((i = rep_of (cc_list cc) b\<^sub>1) \<or> i = rep_of (cc_list cc) b\<^sub>2) \<and>
+      b\<^sub>1 < nr_vars cc \<and> b\<^sub>2 < nr_vars cc \<and> b < nr_vars cc
+    )
+  )
+)"
 
 text \<open>for all pairs of representatives (i, j), Lookup(i, j) is some input equation
 \<open>f(a\<^sub>1, a\<^sub>2)=a\<close> such that i and j are the current respective representatives of \<open>a\<^sub>1\<close> and \<open>a\<^sub>2\<close> whenever
 such an equation exists. Otherwise, Lookup(i, j) is \<bottom>\<close>
 abbreviation lookup_invar_correctness :: "congruence_closure \<Rightarrow> bool"
   where
-    "lookup_invar_correctness cc \<equiv> (\<forall> i < nr_vars cc . (\<forall> j < nr_vars cc . 
-(cc_list cc) ! i = i \<and> (cc_list cc) ! j = j \<longrightarrow>
-lookup cc ! i ! j = None \<or> (\<exists> a\<^sub>1 a\<^sub>2 a . lookup cc ! i ! j = Some (F a\<^sub>1 a\<^sub>2 \<approx> a) \<and> 
-rep_of (cc_list cc) a\<^sub>1 = i \<and> rep_of (cc_list cc) a\<^sub>2 = j)))"
+    "lookup_invar_correctness cc \<equiv> (\<forall> i < nr_vars cc . 
+  (\<forall> j < nr_vars cc .
+    (cc_list cc) ! i = i \<and> (cc_list cc) ! j = j \<longrightarrow> 
+    lookup_valid_element (lookup cc) (cc_list cc) i j 
+  )
+)"
+
 
 definition representativeE :: "congruence_closure \<Rightarrow> equation set"
   where
@@ -118,26 +139,26 @@ abbreviation proof_forest_invar_termination :: "congruence_closure \<Rightarrow>
 
 text \<open>These invariants are needed for the validity proofs:\<close>
 
-abbreviation pending_invar :: "pending_equation list \<Rightarrow> nat list \<Rightarrow> nat \<Rightarrow> bool"
+abbreviation pending_invar :: "pending_equation list \<Rightarrow> nat \<Rightarrow> bool"
   where
-    "pending_invar pe pf n \<equiv> (\<forall> i < length pe . valid_vars_pending (pe ! i) pf n)"
+    "pending_invar pe n \<equiv> (\<forall> i < length pe . valid_vars_pending (pe ! i) n)"
 
 lemma pending_invar_Cons: 
-  "pending_invar (pe # xs) pf n \<longleftrightarrow> pending_invar xs pf n \<and> valid_vars_pending pe pf n"
+  "pending_invar (pe # xs) n \<longleftrightarrow> pending_invar xs n \<and> valid_vars_pending pe n"
 proof
-  show "pending_invar (pe # xs) pf n \<Longrightarrow> pending_invar xs pf n \<and> valid_vars_pending pe pf n"
+  show "pending_invar (pe # xs) n \<Longrightarrow> pending_invar xs n \<and> valid_vars_pending pe n"
     by fastforce
 next 
-  show "pending_invar xs pf n \<and> valid_vars_pending pe pf n \<Longrightarrow> pending_invar (pe # xs) pf n"
+  show "pending_invar xs n \<and> valid_vars_pending pe n \<Longrightarrow> pending_invar (pe # xs) n"
     by (metis in_set_conv_nth set_ConsD)
 qed
 
 lemma pending_left_right_valid: 
-  assumes "pending_invar (pe # xs) pf n"
+  assumes "pending_invar (pe # xs) n"
   shows "right pe < n \<and> left pe < n"
 proof(cases pe)
   case (One x1)
-  have valid: "valid_vars_pending pe pf n" 
+  have valid: "valid_vars_pending pe n" 
     using assms by auto
   with One valid obtain x11 x12 where Constants: "x1 = (x11 \<approx> x12)" 
     by (metis equation.exhaust valid_vars_pending.simps(3))
@@ -145,15 +166,13 @@ proof(cases pe)
   with Constants One valid show ?thesis by auto
 next
   case (Two x21 x22)
-  have valid: "valid_vars_pending pe pf n" 
+  have valid: "valid_vars_pending pe n" 
     using assms by auto
   with valid obtain x211 x212 x213 x221 x222 x223 
     where Function: "x21 = (F x211 x212 \<approx> x213)"  "x22 = (F x221 x222 \<approx> x223)" 
     by (metis Two equation.exhaust valid_vars_pending.simps(4) valid_vars_pending.simps(5))
   then show ?thesis using Two valid by auto
 qed
-
-
 
 text \<open>Here the invariants are put together:\<close>
 
@@ -163,7 +182,7 @@ definition use_list_invar :: "congruence_closure \<Rightarrow> bool"
 
 definition lookup_invar :: "congruence_closure \<Rightarrow> bool"
   where
-    "lookup_invar cc \<equiv> lookup_invar_correctness cc"
+    "lookup_invar cc \<equiv> lookup_invar_correctness cc \<and> quadratic_table (lookup cc)"
 
 definition proof_forest_invar :: "congruence_closure \<Rightarrow> bool"
   where
@@ -181,7 +200,7 @@ definition inv1 :: "congruence_closure \<Rightarrow> bool"
 definition inv2 :: "congruence_closure \<Rightarrow> bool"
   where
     "inv2 cc \<equiv> 
-Congruence_Closure (representativeE cc) = Congruence_Closure (set (input cc))"
+Congruence_Closure (representativeE cc) = Congruence_Closure (input cc)"
 
 text \<open>The union find data structure and the proof forest have the same equivalence classes. \<close>
 abbreviation pf_l_same_eq_classes :: "nat list \<Rightarrow> nat list \<Rightarrow> bool"
@@ -192,6 +211,11 @@ abbreviation pf_l_same_eq_classes :: "nat list \<Rightarrow> nat list \<Rightarr
 definition inv3 :: "congruence_closure \<Rightarrow> bool"
   where
     "inv3 cc \<equiv> pf_l_same_eq_classes (proof_forest cc) (cc_list cc)"
+
+lemma inv3_not_divided: 
+  assumes "i < length (proof_forest cc)" "j < length (proof_forest cc)" "inv3 cc"
+  shows "rep_of (cc_list cc) i = rep_of (cc_list cc) j \<longleftrightarrow> rep_of (proof_forest cc) i = rep_of (proof_forest cc) j"
+  using assms unfolding inv3_def by presburger
 
 lemma inv3_divided: 
   assumes "i < length pf" "j < length pf" 
@@ -209,7 +233,6 @@ abbreviation cc_invar :: "congruence_closure \<Rightarrow> bool"
 lemma cc_invar_initial_cc: "cc_invar (initial_cc n)"
   sorry
 
-
 text \<open>The length of all arrays of congruence_closure is always nr_vars cc\<close>
 lemma length_initial_cc:
   "nr_vars (initial_cc n) = n"
@@ -220,14 +243,19 @@ lemma length_initial_cc:
   by auto
 
 lemma set_lookup_preserves_length:
-  "length t = n \<Longrightarrow> length (set_lookup t a b) = n"
+  "length (set_lookup t a b) = length t"
   apply(induction t a b rule: set_lookup.induct)
   by auto
 
 lemma add_edge_preserves_length:
-  "add_edge_dom (pf, a, b) \<Longrightarrow> length pf = n \<Longrightarrow> length (add_edge pf a b) = n"
+  "add_edge_dom (pf, a, b) \<Longrightarrow> length (add_edge pf a b) = length pf"
   apply(induction pf a b rule: add_edge.pinduct)
   by (simp add: add_edge.psimps)
+
+lemma add_edge_preserves_length':
+  assumes "ufa_invar pf" "a < length pf" "b < length pf" "rep_of pf a \<noteq> rep_of pf b" 
+  shows "length (add_edge pf a b) = length pf"
+  using add_edge_domain add_edge_preserves_length assms by blast
 
 lemma add_label_preserves_length:
   "add_label_dom (pfl, a, b, c) \<Longrightarrow> length pfl = n \<Longrightarrow> length (add_label pfl a b c) = n"
@@ -381,33 +409,14 @@ qed
 
 lemma rep_of_add_edge_invar: 
   assumes "rep_of l a = rep_of l b" "rep_of l x1 \<noteq> rep_of l x2"
-    "ufa_invar l" "a < length l" "b < length l ""x1 < length l ""x2 < length l"
+    "ufa_invar l" "a < length l" "b < length l " "x1 < length l " "x2 < length l"
   shows "rep_of (add_edge l x1 x2) a = rep_of (add_edge l x1 x2) b"
-proof-
-  from assms have dom: "add_edge_dom (l, x1, x2)" 
-    by (simp add: add_edge_domain)
-  from dom assms show ?thesis 
-  proof(induction rule: add_edge.pinduct)
-    case (1 pf e e')
-    then show ?case 
-    proof(cases "pf ! e = e")
-      case True
-      then have "add_edge pf e e' = pf[e := e']" 
-        by (simp add: "1.hyps" add_edge.psimps)
-      then show ?thesis 
-        by (metis "1.prems" rep_of_add_edge_aux)
-    next
-      case False
-      then show ?thesis 
-        by (simp add: "1.prems" rep_of_add_edge_aux)
-    qed
-  qed
-qed
+  by (simp add: assms rep_of_add_edge_aux)
 
 lemma add_edge_inv3_invar:  
   assumes  "pf_l_same_eq_classes pf l" "ufa_invar pf" "ufa_invar l"
-    "a < length pf" "b < length pf" "a < length l" "b < length l"
-    "rep_of l a \<noteq> rep_of l b"
+    "a < length l" "b < length l"
+    "rep_of l a \<noteq> rep_of l b" "length pf = length l"
   shows "pf_l_same_eq_classes (add_edge pf a b) (ufa_union l a b)"
 proof(standard, standard, standard, standard)
   fix i j 
@@ -416,28 +425,255 @@ proof(standard, standard, standard, standard)
     using add_edge_domain by auto
   then have "length (add_edge pf a b) = length pf" 
     by (simp add: add_edge_preserves_length)
-  show "(rep_of (ufa_union l a b) i = rep_of (ufa_union l a b) j) =
+  then show "(rep_of (ufa_union l a b) i = rep_of (ufa_union l a b) j) =
            (rep_of (add_edge pf a b) i = rep_of (add_edge pf a b) j)" 
-  proof (cases "rep_of l i = rep_of l j")
-    case True
-    with assms i_j show ?thesis 
-      by (metis (no_types, lifting) \<open>length (add_edge pf a b) = length pf\<close> rep_of_add_edge rep_of_ufa_union)
-  next
-    case False
-    from rep_of_ufa_union[OF assms(3,6,7)] rep_of_add_edge[OF assms(2,4,5)] assms i_j show ?thesis 
-      sorry
-      by (metis (no_types, lifting) \<open>length (add_edge pf a b) = length pf\<close>)
+    using assms i_j rep_of_add_edge_aux ufa_union_aux by auto
 qed
 
+lemma proof_forest_invar_step: 
+  assumes "proof_forest_invar \<lparr>cc_list = l, use_list = u, lookup = t, proof_forest = pf, pf_labels = pfl, input = ip\<rparr>"
+    "a < length pf" "b < length pf"   "rep_of pf a \<noteq> rep_of pf b"
+  shows "proof_forest_invar
+     (propagate_step l u t pf pfl ip a b pe)"
+  unfolding proof_forest_invar_def using add_edge_ufa_invar_invar
+  using assms proof_forest_invar_def by auto
+
+lemma inv3_step:
+  assumes "inv3 \<lparr>cc_list = l, use_list = u, lookup = t, proof_forest = pf, pf_labels = pfl, input = ip\<rparr>"
+    (is "inv3 ?base")
+    "rep_of pf a \<noteq> rep_of pf b" "ufa_invar pf" "ufa_invar l" "a < length pf" "b < length pf" "length pf = length l"
+  shows "inv3 (propagate_step l u t pf pfl ip a b pe)" (is "inv3 ?step")
+  unfolding inv3_def
+proof(standard, standard, standard, standard)
+  fix i j
+  assume i_j: "i < length (proof_forest ?step)" "j < length (proof_forest ?step)"
+  with add_edge_preserves_length' assms have *:"length (proof_forest ?step) = length (proof_forest ?base)" 
+    by simp
+  with add_edge_preserves_length' assms have "length (cc_list ?step) = length (cc_list ?base)" 
+    by simp
+  with assms * have "(rep_of (cc_list ?base) i = rep_of (cc_list ?base) j) =
+           (rep_of (proof_forest ?base) i = rep_of (proof_forest ?base) j)" unfolding inv3_def using inv3_not_divided 
+    using i_j by presburger
+  with rep_of_add_edge_aux ufa_union_aux assms * i_j inv3_not_divided
+  show "(rep_of (cc_list ?step) i = rep_of (cc_list ?step) j) =
+           (rep_of (proof_forest ?step) i = rep_of (proof_forest ?step) j) " 
+    by (smt (z3) "*" congruence_closure.select_convs(1) congruence_closure.select_convs(4))
+qed
+
+lemma filter_list:
+  assumes "i < length (filter f xs)"
+  shows "f (filter f xs ! i)"
+  by (metis assms length_removeAll_less less_irrefl_nat nth_mem removeAll_filter_not)
+
+lemma filter_list_all:
+  assumes "\<forall> i < length xs . P (xs ! i)"
+  shows "\<forall> i < length (filter f xs) . P ((filter f xs) ! i)"
+proof(standard, standard)
+  fix i
+  assume "i < length (filter f xs)"
+  then have "(filter f xs) ! i \<in> set xs" 
+    by (metis filter_set member_filter nth_mem)
+  then have "\<exists> j < length xs . xs ! j = (filter f xs) ! i" 
+    by (simp add: in_set_conv_nth)
+  then show "P (filter f xs ! i)" 
+    using assms by auto
+qed
+
+lemma filter_lookup_Some:
+  assumes "lookup_invar \<lparr>cc_list = l, use_list = u, lookup = t, proof_forest = pf, pf_labels = pfl, input = ip\<rparr>"
+    "filter (lookup_Some t l) xs ! i = (F a\<^sub>1 a\<^sub>2 \<approx> a)" "ufa_invar l" "a\<^sub>1 < length l" "a\<^sub>2 < length l"
+    "i < length (filter (lookup_Some t l) xs)"
+  obtains b\<^sub>1 b\<^sub>2 b where "lookup_entry t l a\<^sub>1 a\<^sub>2 = Some (F b\<^sub>1 b\<^sub>2 \<approx> b)"
+proof-
+  from assms filter_list have "lookup_entry t l a\<^sub>1 a\<^sub>2 \<noteq> None" 
+    by (metis is_none_simps(1) lookup_Some.simps(1))
+  with assms obtain b\<^sub>1 b\<^sub>2 b where "lookup_entry t l a\<^sub>1 a\<^sub>2 = Some (F b\<^sub>1 b\<^sub>2 \<approx> b)" 
+    unfolding lookup_invar_def 
+    by (metis congruence_closure.select_convs(1) congruence_closure.select_convs(3) rep_of_less_length_l rep_of_min)
+  then show ?thesis ..
+qed
+
+lemma filter_lookup_None:
+  assumes "filter (lookup_None t l) xs ! i = (F a\<^sub>1 a\<^sub>2 \<approx> a)" "i < length (filter (lookup_None t l) xs)"
+  shows "lookup_entry t l a\<^sub>1 a\<^sub>2 = None"
+  by (metis Option.is_none_def assms filter_list lookup_None.simps(1))
+
+lemma use_list_invar_function: 
+  assumes "use_list_invar \<lparr>cc_list = l, use_list = u, lookup = t, proof_forest = pf, pf_labels = pfl, input = ip\<rparr>"
+    "i < length l" "j < length (u ! i)" "l ! i = i"
+  obtains a\<^sub>1 a\<^sub>2 a where "(u ! i) ! j = (F a\<^sub>1 a\<^sub>2 \<approx> a)"
+  using assms unfolding use_list_invar_def by fastforce
+
+lemma filter_use_list_invar_function:
+  assumes "use_list_invar \<lparr>cc_list = l, use_list = u, lookup = t, proof_forest = pf, pf_labels = pfl, input = ip\<rparr>"
+    "i < length l" "j < length (filter f (u ! i))" "l ! i = i"
+  obtains a\<^sub>1 a\<^sub>2 a where "(filter f (u ! i)) ! j = (F a\<^sub>1 a\<^sub>2 \<approx> a)"
+  using use_list_invar_function filter_nth_ex_nth assms  
+  by (metis (no_types, lifting))
+
+lemma use_list_invar_less_n: 
+  assumes "use_list_invar \<lparr>cc_list = l, use_list = u, lookup = t, proof_forest = pf, pf_labels = pfl, input = ip\<rparr>"
+    "i < length l" "j < length (u ! i)" "l ! i = i" "(u ! i) ! j = (F a b \<approx> c)"
+  shows "a < length l" "b < length l" "c < length l"
+  using assms unfolding use_list_invar_def by fastforce+
+
+lemma lookup_invar_less_n:
+  assumes "lookup_invar \<lparr>cc_list = l, use_list = u, lookup = t, proof_forest = pf, pf_labels = pfl, input = ip\<rparr>"
+    "(t ! i) ! j = Some (F f g \<approx> h)" "i < length l" "j < length l" "l ! i = i" "l ! j = j"
+  shows "f < length l" "g < length l" "h < length l"
+  using assms unfolding lookup_invar_def by fastforce+
+
+lemma pending_invar_step:
+  assumes "pending_invar (pe # xs) (length l)" "a = left pe" "ufa_invar l" "length u = length l"
+    "lookup_invar \<lparr>cc_list = l, use_list = u, lookup = t, proof_forest = pf, pf_labels = pfl, input = ip\<rparr>"
+    "use_list_invar \<lparr>cc_list = l, use_list = u, lookup = t, proof_forest = pf, pf_labels = pfl, input = ip\<rparr>" 
+  shows "pending_invar (xs @ map (link_to_lookup t l) (filter (lookup_Some t l) (u ! rep_of l a))) (length l)"
+proof(standard, standard)
+  fix i
+  assume i_valid: "i < length (xs @ map (link_to_lookup t l) (filter (lookup_Some t l) (u ! rep_of l a)))"
+  show "valid_vars_pending ((xs @ map (link_to_lookup t l) (filter (lookup_Some t l) (u ! rep_of l a))) ! i) (length l)"
+  proof(cases "i < length xs")
+    case True
+    with assms show ?thesis 
+      by auto
+  next
+    case False
+    with pending_left_right_valid assms have "a < length l" 
+      by blast
+    then have "rep_of l a < length l" 
+      by (simp add: assms(3) rep_of_less_length_l)
+    have rep_of_a_root: "l ! rep_of l a = rep_of l a" 
+      by (simp add: \<open>a < length l\<close> assms(3) rep_of_root)
+    have i_valid2: "i - length xs < length (filter (lookup_Some t l) (u ! rep_of l a))" 
+      by (metis False i_valid add_diff_inverse_nat add_less_cancel_left length_append length_map)
+    with filter_use_list_invar_function rep_of_a_root False assms obtain c d e 
+      where filter: "(filter (lookup_Some t l) (u ! rep_of l a)) ! (i - length xs) = (F c d \<approx> e)" 
+      by (metis \<open>rep_of l a < length l\<close>)
+    with use_list_invar_less_n[OF assms(6) \<open>rep_of l a < length l\<close>] filter_nth_ex_nth i_valid2 rep_of_a_root 
+    have length_cde: "c < length l" "d < length l""e < length l"
+      by metis+
+    with filter filter_lookup_Some assms obtain f g h where lookup: "lookup_entry t l c d = Some (F f g \<approx> h)"
+      using i_valid2 by blast
+    with lookup_invar_less_n
+    have "f < length l" "g < length l" "h < length l" 
+      using assms length_cde rep_of_less_length_l rep_of_min by meson+
+    with length_cde show ?thesis 
+      by (simp add: False filter i_valid2 lookup nth_append)
+  qed
+qed
+
+lemma set_lookup_valid_input_step:
+  assumes "lookup_invar \<lparr>cc_list = l, use_list = u, lookup = t, proof_forest = pf, pf_labels = pfl, input = ip\<rparr>"
+    "use_list_invar \<lparr>cc_list = l, use_list = u, lookup = t, proof_forest = pf, pf_labels = pfl, input = ip\<rparr>"
+    "ufa_invar l" "length u = length l" "a < length l"
+  shows "set_lookup_valid_input (filter (lookup_None t l) (u ! rep_of l a)) l"
+proof-
+  from assms have "set_lookup_valid_input (u ! rep_of l a) l" 
+    unfolding lookup_invar_def use_list_invar_def
+    by (metis congruence_closure.select_convs(1) congruence_closure.select_convs(2) rep_of_less_length_l rep_of_min)
+  with filter_list_all[where P = "(\<lambda> k . (\<exists>a\<^sub>1 a\<^sub>2 a. k = (F a\<^sub>1 a\<^sub>2 \<approx> a) \<and> a\<^sub>1 < length l \<and> a\<^sub>2 < length l \<and> a < length l))"] 
+  show ?thesis by blast
+qed
+
+lemma lookup_invar_step: 
+  assumes "lookup_invar \<lparr>cc_list = l, use_list = u, lookup = t, proof_forest = pf, pf_labels = pfl, input = ip\<rparr>"
+    (is "lookup_invar ?base") 
+    "use_list_invar \<lparr>cc_list = l, use_list = u, lookup = t, proof_forest = pf, pf_labels = pfl, input = ip\<rparr>"
+    "ufa_invar l" "a < length l" "b < length l" "length t = length l" "length u = length l"
+  shows "lookup_invar (propagate_step l u t pf pfl ip a b pe)" (is "lookup_invar ?step")
+  unfolding lookup_invar_def proof(standard, standard, standard, standard, standard, standard)
+  fix i j
+  assume i_j: "i < nr_vars ?step" "j < nr_vars ?step" "cc_list ?step ! i = i \<and> cc_list ?step ! j = j"
+  have step_list: "cc_list ?step = (ufa_union l a b)"
+    "lookup ?step = set_lookup t (filter (lookup_None t l) (u ! rep_of l a)) l"
+    by auto
+  with i_j ufa_union_root assms have *: "l ! i = i \<and> l ! j = j"
+    by metis
+  from assms have 1: "lookup_valid_element t l i j" unfolding lookup_invar_def 
+    using "*" i_j by auto
+  from set_lookup_valid_input_step assms have 2: "set_lookup_valid_input (filter (lookup_None t l) (u ! rep_of l a)) l"
+    by blast
+  with * set_lookup_valid assms i_j 1 2 step_list have "lookup_valid_element (lookup ?step) l i j"
+    unfolding lookup_invar_def by auto
+  with i_j ufa_union_lookup_valid assms show "lookup_valid_element (lookup ?step) (cc_list ?step) i j" 
+    by auto
+next
+  from set_lookup_valid_length show "quadratic_table (lookup (propagate_step l u t pf pfl ip a b pe))"
+    using assms lookup_invar_def by auto
+qed
+
+lemma use_list_invar_step: 
+  assumes "lookup_invar \<lparr>cc_list = l, use_list = u, lookup = t, proof_forest = pf, pf_labels = pfl, input = ip\<rparr>"
+    (is "lookup_invar ?base") 
+    "use_list_invar \<lparr>cc_list = l, use_list = u, lookup = t, proof_forest = pf, pf_labels = pfl, input = ip\<rparr>"
+    "ufa_invar l" "a < length l" "b < length l" "length t = length l" "length u = length l"
+  shows "use_list_invar (propagate_step l u t pf pfl ip a b pe)" (is "use_list_invar ?step")
+  unfolding use_list_invar_def proof(standard, standard,standard, standard, standard)
+  fix i j 
+  assume i_j: "i < nr_vars ?step" 
+    "j < length (use_list ?step ! i)"
+    "cc_list ?step ! i = i"
+  consider (rep_of_a) "i = rep_of l a" "rep_of l a \<noteq> rep_of l b" | (rep_of_b) "i = rep_of l b" 
+    | (none) "i \<noteq> rep_of l a \<and> i \<noteq> rep_of l b" 
+    by blast
+  then show "\<exists>b\<^sub>1 b\<^sub>2 ba. use_list ?step ! i ! j = F b\<^sub>1 b\<^sub>2 \<approx> ba \<and> (i = rep_of (cc_list ?step) b\<^sub>1 \<or>
+               i = rep_of (cc_list ?step) b\<^sub>2) \<and>
+               b\<^sub>1 < nr_vars ?step \<and> b\<^sub>2 < nr_vars ?step \<and> ba < nr_vars ?step"
+  proof(cases)
+    case rep_of_a
+    then have "use_list ?step ! i = []" 
+      using i_j by auto
+    then show ?thesis 
+      using i_j(2) len_greater_imp_nonempty by blast
+  next
+    case rep_of_b
+    then have *: "use_list ?step ! i = u ! rep_of l b @ filter (lookup_None t l) (u ! rep_of l a)" 
+      using assms(7) i_j(1) by auto
+    have rep_a: "rep_of (cc_list ?step) a = rep_of l b" 
+      by (simp add: assms(3) assms(4) assms(5) ufa_union_aux)
+    have rep_b: "rep_of (cc_list ?step) b = rep_of l b" 
+      by (simp add: assms(3) assms(4) assms(5) ufa_union_aux)
+    then show ?thesis proof(cases "j < length (u ! rep_of l b)")
+      case True
+      with * have "use_list ?step ! i ! j = u ! i ! j" 
+        by (simp add: rep_of_b)
+      with rep_a rep_b assms show ?thesis unfolding use_list_invar_def 
+        by (metis True congruence_closure.select_convs(1) congruence_closure.select_convs(2) i_j(1) length_list_update rep_of_b rep_of_min rep_of_ufa_union_invar)
+    next
+      case False
+      with * have 
+        use_list_step: "use_list ?step ! i ! j = (filter (lookup_None t l) (u ! rep_of l a)) ! (j - length (u ! rep_of l b))"
+        by (simp add: nth_append)
+      from i_j have **: "j < length (u ! rep_of l b) + length (filter (lookup_None t l) (u ! rep_of l a))" 
+        by (metis "*" length_append)
+      then have "(j - length (u ! rep_of l b)) < length (filter (lookup_None t l) (u ! rep_of l a))" 
+        using False by linarith
+      with ** filter_set member_filter nth_mem have "use_list ?step ! i ! j \<in> set (u ! rep_of l a)"
+        by (metis use_list_step)
+      then obtain k where "use_list ?step ! i ! j = (u ! rep_of l a) ! k" "k < length (u ! rep_of l a)"
+        by (metis in_set_conv_nth)
+      with rep_a rep_b assms show ?thesis unfolding use_list_invar_def  
+        by (metis congruence_closure.select_convs(1) congruence_closure.select_convs(2) length_list_update rep_of_b rep_of_bound rep_of_min rep_of_ufa_union_invar)
+    qed
+  next
+    case none
+    then have "use_list ?step ! i = u ! i" 
+      by auto
+    with assms show ?thesis unfolding use_list_invar_def 
+      by (metis congruence_closure.select_convs(1,2) i_j length_list_update none nth_list_update_neq rep_of_iff rep_of_ufa_union_invar ufa_union_invar)
+  qed
+qed
 
 lemma propagate_preserves_length_proof_forest:
-  assumes "propagate_dom (a, cc)" "length (proof_forest cc) = n" "length (cc_list cc) = n" "proof_forest_invar cc"
-    "pending_invar a (proof_forest cc) n" "inv3 cc"
+  assumes "propagate_dom (a, cc)" 
+    "length (proof_forest cc) = n" "length (cc_list cc) = n" "length (use_list cc) = n" "length (lookup cc) = n"
+    "proof_forest_invar cc" "lookup_invar cc" "use_list_invar cc"
+    "ufa_invar (cc_list cc)" "pending_invar a n" "inv3 cc"
   shows "length (proof_forest (propagate a cc)) = n"
   using assms proof(induction a cc rule: propagate.pinduct)
   case (1 cc)
   then show ?case 
-    by (simp add: propagate.psimps(1))
+    by simp
 next
   case (2 pe xs l u t pf pfl ip) 
   define a where "a = left pe"
@@ -452,36 +688,49 @@ next
          \<lparr>cc_list = l, use_list = u, lookup = t, proof_forest = pf, pf_labels = pfl, input = ip\<rparr>
   = propagate xs \<lparr>cc_list = l, use_list = u, lookup = t, proof_forest = pf, pf_labels = pfl, input = ip\<rparr>" using a_def b_def propagate_simps
       by (metis "2.hyps" propagate_simp2')
-    moreover have "pending_invar xs
-     (proof_forest \<lparr>cc_list = l, use_list = u, lookup = t, proof_forest = pf, pf_labels = pfl, input = ip\<rparr>) n"
-      using "2.prems"(3) pending_invar_Cons by blast
+    moreover have "pending_invar xs n"
+      using "2.prems" pending_invar_Cons by blast
     ultimately show ?thesis using 2 True a_def b_def by metis
-next
-  case False
-  with 2 have "rep_of pf a \<noteq> rep_of pf b" 
-    by (metis "*"(1) a_b(1) a_b(2) inv3_divided)
-  with add_edge_domain a_b * have dom: "add_edge_dom (pf, a, b)"
-    by metis
-  with 2 add_edge_preserves_length * have "length (add_edge pf a b) = n"
-    by presburger
-  from * a_b dom add_edge_ufa_invar_invar have "ufa_invar (add_edge pf a b)" 
-    by (simp add: \<open>rep_of pf a \<noteq> rep_of pf b\<close>)
-  have " pending_invar (xs @ map (link_to_lookup t) (filter (lookup_Some t) (u ! rep_of l a))) (add_edge pf a b)
-     n "sorry
-  have "propagate (pe # xs)
-         \<lparr>cc_list = l, use_list = u, lookup = t, proof_forest = pf, pf_labels = pfl, input = ip\<rparr>
-              = propagate (xs @ (map (link_to_lookup t) (filter (lookup_Some t) (u ! rep_of l a))))
-              \<lparr>cc_list = ufa_union l a b, 
-              use_list = (u[rep_of l a := []])[rep_of l b := (u ! rep_of l b) @ (filter (lookup_None t) (u ! rep_of l a))], 
-              lookup = set_lookup t (filter (lookup_None t) (u ! rep_of l a)) l,
-              proof_forest = add_edge pf a b, pf_labels = add_label pfl pf a pe, input = ip\<rparr>" 
-    using "2.hyps" False a_def b_def propagate_simp3 by blast
-  with False 2 propagate_simps show ?thesis unfolding a_def b_def 
-  proof_forest_invar_def inv3_def
-congruence_closure.select_convs  sorry
-qed
-
-  
+  next
+    case False
+    with 2 have rep_of_pf: "rep_of pf a \<noteq> rep_of pf b" 
+      by (metis "*"(1) a_b(1) a_b(2) inv3_divided)
+    with add_edge_domain a_b * have dom: "add_edge_dom (pf, a, b)"
+      by metis
+    with 2 add_edge_preserves_length * have length_add_edge: "length (add_edge pf a b) = n"
+      by presburger
+    from 2(5) have length_ufa_union: "length (ufa_union l a b) = n"
+      by force
+    from * a_b dom add_edge_ufa_invar_invar have "ufa_invar (add_edge pf a b)" 
+      by (simp add: \<open>rep_of pf a \<noteq> rep_of pf b\<close>)
+    have "length l = n" "ufa_invar l"
+      using length_ufa_union apply fastforce using 2(11) 
+      by simp
+    with pending_invar_step[of pe xs l a u] 2 a_def have pending_invar: "pending_invar (xs @ map (link_to_lookup t l) (filter (lookup_Some t l) (u ! rep_of l a))) (length l)"
+      by (metis congruence_closure.select_convs(2))
+    from proof_forest_invar_step "2.prems" have proof_forest_invar: 
+      "proof_forest_invar (propagate_step l u t pf pfl ip a b pe)" 
+      using \<open>rep_of pf a \<noteq> rep_of pf b\<close> a_b add_edge_preserves_length dom length_add_edge by presburger
+    have "ufa_invar pf" "ufa_invar l" "a < length pf" "b < length pf" "length pf = length l"
+      using * a_b \<open>ufa_invar l\<close> \<open>length l = n\<close> by simp_all
+    from inv3_step[OF 2(13) rep_of_pf this] have inv3: "inv3 (propagate_step l u t pf pfl ip a b pe)" by blast
+    from "2.prems" have "a < length l" "b < length l" "length t = length l" "length u = length l" 
+      by (auto simp add:  \<open>length l = n\<close> a_b) 
+    with lookup_invar_step 2 have lookup_invar: "lookup_invar (propagate_step l u t pf pfl ip a b pe)"
+      using \<open>ufa_invar l\<close> by presburger
+    from use_list_invar_step have use_list_invar: "use_list_invar (propagate_step l u t pf pfl ip a b pe)"
+      by (simp add: "2.prems" \<open>a < length l\<close> \<open>b < length l\<close> \<open>length t = length l\<close> \<open>length u = length l\<close> \<open>ufa_invar l\<close> )
+    have "ufa_invar (ufa_union l a b)" "length (lookup (propagate_step l u t pf pfl ip a b pe)) = n"
+      using \<open>a < length pf\<close> \<open>b < length pf\<close> \<open>length pf = length l\<close> \<open>ufa_invar l\<close> ufa_union_invar
+      by (simp_all add: \<open>length l = n\<close> \<open>length t = length l\<close> set_lookup_preserves_length)
+    with 2(3)[OF a_def b_def False _ _ _ _ proof_forest_invar lookup_invar use_list_invar] False proof_forest_invar inv3 length_add_edge length_ufa_union pending_invar
+    have "length (proof_forest
+       (propagate (xs @ map (link_to_lookup t l) (filter (lookup_Some t l) (u ! rep_of l a)))
+         (propagate_step l u t pf pfl ip a b pe))) = n" 
+      by (metis "2.prems"(3) congruence_closure.select_convs(1,2,4) length_list_update)
+    with False 2 propagate_simps show ?thesis unfolding a_def b_def
+      by presburger
+  qed
 qed
 
 lemma propagate_preserves_length_pf_labels:
